*****

GIT.v
@@ -431,6 +431,589 @@ End Chapter1.
 
 Section Chapter2.
 
+Definition vr : Set :=
+  nat
+.
+
+Inductive tm : Set :=
+| ivar_tm : vr -> tm
+| zero_tm : tm
+| succ_tm : tm -> tm
+| plus_tm : tm -> tm -> tm
+| mult_tm : tm -> tm -> tm
+| expo_tm : tm -> tm -> tm
+.
+
+Inductive form : Set :=
+| eqn_form : tm -> tm -> form
+| leq_form : tm -> tm -> form
+| neg_form : form -> form
+| imp_form : form -> form -> form
+| all_form : vr -> form -> form
+.
+
+Lemma vr_eq_dec :
+  forall x1 : vr,
+  forall x2 : vr,
+  {x1 = x2} + {x1 <> x2}.
+Proof.
+  apply Nat.eq_dec.
+Qed.
+
+Fixpoint occursFreeIn_tm (z : vr) (t : tm) : bool :=
+  match t with
+  | ivar_tm x => if vr_eq_dec z x then true else false
+  | zero_tm => false
+  | succ_tm t1 => occursFreeIn_tm z t1
+  | plus_tm t1 t2 => occursFreeIn_tm z t1 || occursFreeIn_tm z t2
+  | mult_tm t1 t2 => occursFreeIn_tm z t1 || occursFreeIn_tm z t2
+  | expo_tm t1 t2 => occursFreeIn_tm z t1 || occursFreeIn_tm z t2
+  end
+.
+
+Fixpoint occursFreeIn_form (z : vr) (f : form) : bool :=
+  match f with
+  | eqn_form t1 t2 => occursFreeIn_tm z t1 || occursFreeIn_tm z t2
+  | leq_form t1 t2 => occursFreeIn_tm z t1 || occursFreeIn_tm z t2
+  | neg_form f1 => occursFreeIn_form z f1
+  | imp_form f1 f2 => occursFreeIn_form z f1 || occursFreeIn_form z f2
+  | all_form x f1 => if vr_eq_dec z x then false else occursFreeIn_form z f1
+  end
+.
+
+Fixpoint getFreeVars_tm (t : tm) : list vr :=
+  match t with
+  | ivar_tm x => [x]
+  | zero_tm => []
+  | succ_tm t1 => getFreeVars_tm t1
+  | plus_tm t1 t2 => getFreeVars_tm t1 ++ getFreeVars_tm t2
+  | mult_tm t1 t2 => getFreeVars_tm t1 ++ getFreeVars_tm t2
+  | expo_tm t1 t2 => getFreeVars_tm t1 ++ getFreeVars_tm t2
+  end
+.
+
+Theorem the_rule_of_getFreeVars_tm :
+  forall t : tm,
+  forall x : vr,
+  In x (getFreeVars_tm t) <-> occursFreeIn_tm x t = true.
+Proof.
+  intros t; induction t.
+  - intros vr; simpl; constructor.
+    + intros H; destruct H.
+      { subst.
+        destruct (vr_eq_dec vr vr).
+        - reflexivity.
+        - contradiction.
+      }
+      { contradiction.
+      }
+    + intros H; destruct (vr_eq_dec vr v).
+      { rewrite e; left; reflexivity.
+      }
+      { inversion H.
+      }
+  - intros vr; simpl; constructor.
+    + tauto.
+    + intros H; inversion H.
+  - intros vr; simpl; apply IHt.
+  - intros vr; simpl; rewrite orb_true_iff; rewrite in_app_iff; rewrite IHt1; rewrite IHt2; reflexivity.
+  - intros vr; simpl; rewrite orb_true_iff; rewrite in_app_iff; rewrite IHt1; rewrite IHt2; reflexivity.
+  - intros vr; simpl; rewrite orb_true_iff; rewrite in_app_iff; rewrite IHt1; rewrite IHt2; reflexivity.
+Qed.
+
+Fixpoint getFreeVars_form (f : form) : list vr :=
+  match f with
+  | eqn_form t1 t2 => getFreeVars_tm t1 ++ getFreeVars_tm t2
+  | leq_form t1 t2 => getFreeVars_tm t1 ++ getFreeVars_tm t2
+  | neg_form f1 => getFreeVars_form f1
+  | imp_form f1 f2 => getFreeVars_form f1 ++ getFreeVars_form f2
+  | all_form x f1 => remove vr_eq_dec x (getFreeVars_form f1)
+  end
+.
+
+Theorem the_rule_of_getFreeVars_form :
+  forall f : form,
+  forall x : vr,
+  In x (getFreeVars_form f) <-> occursFreeIn_form x f = true.
+Proof.
+  intros f; induction f.
+  - intros vr; simpl; rewrite orb_true_iff; rewrite in_app_iff; rewrite the_rule_of_getFreeVars_tm; rewrite the_rule_of_getFreeVars_tm; reflexivity.
+  - intros vr; simpl; rewrite orb_true_iff; rewrite in_app_iff; rewrite the_rule_of_getFreeVars_tm; rewrite the_rule_of_getFreeVars_tm; reflexivity.
+  - intros vr; simpl; apply IHf.
+  - intros vr; simpl; rewrite orb_true_iff; rewrite in_app_iff; rewrite IHf1; rewrite IHf2; reflexivity.
+  - intros vr; simpl; constructor.
+    + intros H.
+      assert (In vr (getFreeVars_form f) /\ vr <> v).
+      { apply (in_remove vr_eq_dec (getFreeVars_form f) vr v); apply H.
+      }
+      destruct H0 as [H0 H1]; destruct (vr_eq_dec vr v).
+      { contradiction H1.
+      }
+      { apply IHf; apply H0.
+      }
+    + intros H; destruct (vr_eq_dec vr v).
+      { inversion H.
+      }
+      { apply in_in_remove.
+        - apply n.
+        - apply IHf; apply H.
+      }
+Qed.
+
+Definition value_assignment : Set :=
+  vr -> nat
+.
+
+Fixpoint eval_tm (va : value_assignment) (t : tm) : nat :=
+  match t with
+  | ivar_tm x => va x
+  | zero_tm => 0
+  | succ_tm t1 => S (eval_tm va t1)
+  | plus_tm t1 t2 => eval_tm va t1 + eval_tm va t2
+  | mult_tm t1 t2 => eval_tm va t1 * eval_tm va t2
+  | expo_tm t1 t2 => (eval_tm va t1)^(eval_tm va t2)
+  end
+.
+
+Lemma eval_tm_extensionality :
+  forall t : tm,
+  forall va1 : value_assignment,
+  forall va2 : value_assignment,
+  (forall x : vr, occursFreeIn_tm x t = true -> va1 x = va2 x) ->
+  eval_tm va1 t = eval_tm va2 t.
+Proof.
+  intros t; induction t.
+  - simpl; intros va1 va2 H; apply H; destruct (vr_eq_dec v v).
+    + reflexivity.
+    + contradiction.
+  - simpl; intros va1 va2 H.
+    reflexivity.
+  - simpl; intros va1 va2 H.
+    rewrite (IHt va1 va2).
+    reflexivity.
+    apply H.
+  - simpl; intros va1 va2 H.
+    rewrite (IHt1 va1 va2).
+    rewrite (IHt2 va1 va2).
+    reflexivity.
+    intros x H0; apply H; apply orb_true_iff; tauto.
+    intros x H0; apply H; apply orb_true_iff; tauto.
+  - simpl; intros va1 va2 H.
+    rewrite (IHt1 va1 va2).
+    rewrite (IHt2 va1 va2).
+    reflexivity.
+    intros x H0; apply H; apply orb_true_iff; tauto.
+    intros x H0; apply H; apply orb_true_iff; tauto.
+  - simpl; intros va1 va2 H.
+    rewrite (IHt1 va1 va2).
+    rewrite (IHt2 va1 va2).
+    reflexivity.
+    intros x H0; apply H; apply orb_true_iff; tauto.
+    intros x H0; apply H; apply orb_true_iff; tauto.
+Qed.
+
+Fixpoint eval_form (va : value_assignment) (f : form) : Prop :=
+  match f with
+  | eqn_form t1 t2 => eval_tm va t1 = eval_tm va t2
+  | leq_form t1 t2 => eval_tm va t1 <= eval_tm va t2
+  | neg_form f1 => ~ eval_form va f1
+  | imp_form f1 f2 => eval_form va f1 -> eval_form va f2
+  | all_form x f1 => forall val : nat, eval_form (fun z : vr => if vr_eq_dec x z then val else va z) f1
+  end
+.
+
+Lemma eval_form_extensionality :
+  forall f : form,
+  forall va1 : value_assignment,
+  forall va2 : value_assignment,
+  (forall x : vr, occursFreeIn_form x f = true -> va1 x = va2 x) ->
+  eval_form va1 f <-> eval_form va2 f.
+Proof.
+  intros f; induction f.
+  - simpl; intros va1 va2 H.
+    rewrite (eval_tm_extensionality t va1 va2).
+    rewrite (eval_tm_extensionality t0 va1 va2).
+    reflexivity.
+    intros x H0; apply H; apply orb_true_iff; tauto.
+    intros x H0; apply H; apply orb_true_iff; tauto.
+  - simpl; intros va1 va2 H.
+    rewrite (eval_tm_extensionality t va1 va2).
+    rewrite (eval_tm_extensionality t0 va1 va2).
+    reflexivity.
+    intros x H0; apply H; apply orb_true_iff; tauto.
+    intros x H0; apply H; apply orb_true_iff; tauto.
+  - simpl; intros va1 va2 H.
+    rewrite (IHf va1 va2).
+    reflexivity.
+    intros x H0; apply H; tauto.
+  - simpl; intros va1 va2 H.
+    rewrite (IHf1 va1 va2).
+    rewrite (IHf2 va1 va2).
+    reflexivity.
+    intros x H0; apply H; apply orb_true_iff; tauto.
+    intros x H0; apply H; apply orb_true_iff; tauto.
+  - simpl; intros va1 va2 H.
+    cut (
+      forall n : nat,
+      eval_form (fun z : vr => if vr_eq_dec v z then n else va1 z) f <->  eval_form (fun z : vr => if vr_eq_dec v z then n else va2 z) f
+    ).
+    { constructor.
+      - intros H1 n; apply H0; apply H1.
+      - intros H1 n; apply H0; apply H1.
+    }
+    intros n.
+    rewrite (IHf (fun z : vr => if vr_eq_dec v z then n else va1 z) (fun z : vr => if vr_eq_dec v z then n else va2 z)).
+    reflexivity.
+    intros x H0; destruct (vr_eq_dec v x).
+    { reflexivity.
+    }
+    { apply H.
+      destruct (vr_eq_dec x v).
+      - contradiction n0; rewrite e; reflexivity.
+      - apply H0.
+    }
+Qed.
+
+Fixpoint make_numeral (n : nat) : tm :=
+  match n with
+  | 0 => zero_tm
+  | S n => succ_tm (make_numeral n)
+  end
+.
+
+Lemma eval_tm_make_numeral :
+  forall n : nat,
+  forall va : value_assignment,
+  eval_tm va (make_numeral n) = n.
+Proof.
+  intros n; induction n.
+  - simpl; intros va; reflexivity.
+  - simpl; intros va; rewrite IHn; reflexivity.
+Qed.
+
+Definition substitution : Set :=
+  list (vr * tm)
+.
+
+Fixpoint substitute_vr (sigma : substitution) (x : vr) : tm :=
+  match sigma with
+  | [] => ivar_tm x
+  | (x1, tm1) :: sigma' => if vr_eq_dec x x1 then tm1 else substitute_vr sigma' x
+  end
+.
+
+Fixpoint substitute_tm (sigma : substitution) (t : tm) : tm :=
+  match t with
+  | ivar_tm x => substitute_vr sigma x
+  | zero_tm => zero_tm
+  | succ_tm t1 => succ_tm (substitute_tm sigma t1)
+  | plus_tm t1 t2 => plus_tm (substitute_tm sigma t1) (substitute_tm sigma t2)
+  | mult_tm t1 t2 => mult_tm (substitute_tm sigma t1) (substitute_tm sigma t2)
+  | expo_tm t1 t2 => expo_tm (substitute_tm sigma t1) (substitute_tm sigma t2)
+  end
+.
+
+Theorem substitute_tm_preserves_eval_tm :
+  forall t : tm,
+  forall sigma : substitution,
+  forall va : value_assignment,
+  eval_tm (fun z : vr => eval_tm va (substitute_vr sigma z)) t = eval_tm va (substitute_tm sigma t).
+Proof.
+  intros t; induction t.
+  - intros sigma va; simpl; reflexivity.
+  - intros sigma va; simpl; reflexivity.
+  - intros sigma va; simpl; rewrite IHt; reflexivity.
+  - intros sigma va; simpl; rewrite IHt1; rewrite IHt2; reflexivity.
+  - intros sigma va; simpl; rewrite IHt1; rewrite IHt2; reflexivity.
+  - intros sigma va; simpl; rewrite IHt1; rewrite IHt2; reflexivity.
+Qed.
+
+Definition getMaxNumOfFreeVars_tm (t : tm) : vr :=
+  fold_right_max_0 (getFreeVars_tm t)
+.
+Lemma getMaxNumOfFreeVars_tm_lt :
+  forall t : tm,
+  forall x : vr,
+  getMaxNumOfFreeVars_tm t < x ->
+  occursFreeIn_tm x t = false.
+Proof.
+  unfold getMaxNumOfFreeVars_tm; intros t; induction t.
+  - simpl; intros x H; destruct (vr_eq_dec x v).
+    + lia.
+    + reflexivity.
+  - simpl; intros x H; tauto.
+  - simpl; intros x H; apply IHt; apply H.
+  - simpl; intros x H; apply orb_false_iff; rewrite fold_right_max_0_app in H; constructor.
+    + apply IHt1; lia.
+    + apply IHt2; lia.
+  - simpl; intros x H; apply orb_false_iff; rewrite fold_right_max_0_app in H; constructor.
+    + apply IHt1; lia.
+    + apply IHt2; lia.
+  - simpl; intros x H; apply orb_false_iff; rewrite fold_right_max_0_app in H; constructor.
+    + apply IHt1; lia.
+    + apply IHt2; lia.
+Qed.
+
+Definition isFreshVarIn_substitute_tm (sigma : substitution) (z : vr) (t : tm) : Prop :=
+  forallb (fun x : vr => negb (occursFreeIn_tm z (substitute_vr sigma x))) (getFreeVars_tm t) = true
+.
+
+Definition isFreshVarIn_substitute_form (sigma : substitution) (z : vr) (f : form) : Prop :=
+  forallb (fun x : vr => negb (occursFreeIn_tm z (substitute_vr sigma x))) (getFreeVars_form f) = true
+.
+
+Definition chi (sigma : substitution) (f : form) : vr :=
+  S (fold_right_max_0 (map (fun x : vr => getMaxNumOfFreeVars_tm (substitute_vr sigma x)) (getFreeVars_form f)))
+.
+
+Theorem the_rule_of_chi :
+  forall f : form,
+  forall sigma : substitution,
+  isFreshVarIn_substitute_form sigma (chi sigma f) f.
+Proof.
+  assert ( claim1 :
+    forall sigma : substitution,
+    forall f : form,
+    forall x : vr,
+    occursFreeIn_form x f = true ->
+    occursFreeIn_tm (chi sigma f) (substitute_vr sigma x) = false
+  ).
+  { intros sigma f x H.
+    assert (getMaxNumOfFreeVars_tm (substitute_vr sigma x) < chi sigma f).
+    { unfold chi; unfold fold_right_max_0.
+      cut (fold_right max 0 (map (fun z : vr => getMaxNumOfFreeVars_tm (substitute_vr sigma z)) (getFreeVars_form f)) >= getMaxNumOfFreeVars_tm (substitute_vr sigma x)).
+      { lia.
+      }
+      rewrite <- the_rule_of_getFreeVars_form in H.
+      apply fold_right_max_0_in; apply in_map_iff.
+      exists x; constructor.
+      - reflexivity.
+      - apply H.
+    }
+    apply getMaxNumOfFreeVars_tm_lt; apply H0.
+  }
+  unfold isFreshVarIn_substitute_form; intros f sigma; apply forallb_true_iff.
+  intros x H; apply negb_true_iff; apply claim1; apply the_rule_of_getFreeVars_form; apply H.
+Qed.
+
+Fixpoint substitute_form (sigma : substitution) (f : form) : form :=
+  match f with
+  | eqn_form t1 t2 => eqn_form (substitute_tm sigma t1) (substitute_tm sigma t2)
+  | leq_form t1 t2 => leq_form (substitute_tm sigma t1) (substitute_tm sigma t2)
+  | neg_form f1 => neg_form (substitute_form sigma f1)
+  | imp_form f1 f2 => imp_form (substitute_form sigma f1) (substitute_form sigma f2)
+  | all_form x f1 =>
+    let z : vr := chi sigma f in
+    all_form z (substitute_form ((x, ivar_tm z) :: sigma) f1)
+  end
+.
+
+Theorem substitute_form_preserves_eval_form :
+  forall f : form,
+  forall sigma : substitution,
+  forall va : value_assignment,
+  eval_form (fun z : vr => eval_tm va (substitute_vr sigma z)) f <-> eval_form va (substitute_form sigma f).
+Proof.
+  intros f; induction f.
+  - intros sigma va; simpl.
+    rewrite substitute_tm_preserves_eval_tm; rewrite substitute_tm_preserves_eval_tm; reflexivity.
+  - intros sigma va; simpl.
+    rewrite substitute_tm_preserves_eval_tm; rewrite substitute_tm_preserves_eval_tm; reflexivity.
+  - intros sigma va; simpl.
+    rewrite IHf; reflexivity.
+  - intros sigma va; simpl.
+    rewrite IHf1; rewrite IHf2; reflexivity.
+  - intros sigma va. simpl.
+    cut (
+      forall n : nat,
+      eval_form (fun z : vr => if vr_eq_dec v z then n else eval_tm va (substitute_vr sigma z)) f <-> eval_form (fun z : vr => if vr_eq_dec (chi sigma (all_form v f)) z then n else va z) (substitute_form ((v, ivar_tm (chi sigma (all_form v f))) :: sigma) f)
+    ).
+    { intros H; constructor.
+      - intros H0 n; apply H; apply H0.
+      - intros H0 n; apply H; apply H0.
+    }
+    intros n; rewrite <- (IHf ((v, ivar_tm (chi sigma (all_form v f))) :: sigma) (fun z : vr => if vr_eq_dec (chi sigma (all_form v f)) z then n else va z)); apply eval_form_extensionality.
+    intros x H; simpl; destruct (vr_eq_dec v x).
+    { destruct (vr_eq_dec x v).
+      - simpl; destruct (vr_eq_dec (chi sigma (all_form v f)) (chi sigma (all_form v f))).
+        + reflexivity.
+        + contradiction.
+      - contradiction n0; rewrite e; reflexivity.
+    }
+    { destruct (vr_eq_dec x v).
+      - contradiction n0; rewrite e; reflexivity.
+      - apply eval_tm_extensionality.
+        intros x' H0; destruct (vr_eq_dec (chi sigma (all_form v f)) x').
+        + subst.
+          assert (isFreshVarIn_substitute_form sigma (chi sigma (all_form v f)) (all_form v f)).
+            apply the_rule_of_chi.
+          unfold isFreshVarIn_substitute_form in H1; rewrite forallb_true_iff in H1.
+          assert (negb (occursFreeIn_tm (chi sigma (all_form v f)) (substitute_vr sigma x)) = true).
+          { apply H1; apply the_rule_of_getFreeVars_form; simpl; destruct (vr_eq_dec x v).
+            - contradiction.
+            - tauto. 
+          }
+          rewrite H0 in H2; inversion H2.
+        + reflexivity.
+    }
+Qed.
+
+Lemma substitute_tm_make_numeral :
+  forall n : nat,
+  forall sigma : substitution,
+  substitute_tm sigma (make_numeral n) = make_numeral n.
+Proof.
+  intros n; induction n.
+  - intros sigma; simpl; reflexivity.
+  - intros sigma; simpl; rewrite (IHn sigma); reflexivity.
+Qed.
+
+Ltac simpl_eval_tm_make_numeral :=
+  repeat (rewrite substitute_tm_make_numeral); repeat (rewrite eval_tm_make_numeral)
+.
+
+Ltac simpl_in_eval_tm_make_numeral H := 
+  repeat (rewrite substitute_tm_make_numeral in H); repeat (rewrite eval_tm_make_numeral in H)
+.
+
+Lemma occursFreeIn_tm_make_numeral :
+  forall val : nat,
+  forall x : vr,
+  occursFreeIn_tm x (make_numeral val) = false.
+Proof.
+  intros val; induction val.
+  - intros x; simpl; reflexivity.
+  - intros x; simpl; rewrite (IHval x); reflexivity.
+Qed.
+
+Ltac simplify_make_numeral := repeat (rewrite substitute_tm_make_numeral); repeat (apply occursFreeIn_tm_make_numeral).
+
+Lemma vr_eq_dec_is_Nat_eq_dec {A : Type} :
+  forall x1 : A,
+  forall x2 : A,
+  forall z1 : vr,
+  forall z2 : vr,
+  (if vr_eq_dec z1 z2 then x1 else x2) = (if Nat.eq_dec z1 z2 then x1 else x2).
+Proof.
+  intros x1 x2 z1 z2.
+  destruct (vr_eq_dec z1 z2).
+  - destruct (Nat.eq_dec z1 z2).
+    + reflexivity.
+    + contradiction.
+  - destruct (Nat.eq_dec z1 z2).
+    + contradiction.
+    + reflexivity.
+Qed.
+
+Ltac eval_vr_eq_dec :=
+  repeat (rewrite vr_eq_dec_is_Nat_eq_dec; simpl)
+.
+
+Ltac eval_in_vr_eq_dec H :=
+  repeat (rewrite vr_eq_dec_is_Nat_eq_dec in H; simpl in H)
+.
+
+Fixpoint relation_of_arity (n : nat) : Type :=
+  match n with
+  | 0 => Prop
+  | S n' => nat -> relation_of_arity n'
+  end
+.
+
+Fixpoint lift_relation (n : nat) : relation_of_arity (S n) -> nat -> relation_of_arity n :=
+  match n as n0 return relation_of_arity (S n0) -> nat -> relation_of_arity n0 with
+  | 0 =>
+    fun pred : nat -> Prop =>
+    fun val : nat =>
+    pred val
+  | S n' =>
+    fun pred : nat -> nat -> relation_of_arity n' =>
+    fun val : nat =>
+    fun val' : nat =>
+    lift_relation n' (pred val') val 
+  end
+.
+
+Fixpoint express_relation (n : nat) : form -> relation_of_arity n -> Prop :=
+  match n as n0 return form -> relation_of_arity n0 -> Prop with
+  | 0 =>
+    fun f : form =>
+    fun pred : Prop =>
+    (forall x : vr, occursFreeIn_form x f = false) /\ (pred <-> forall va : value_assignment, eval_form va f)
+  | S n' =>
+    fun f : form =>
+    fun pred : nat -> relation_of_arity n' =>
+    forall val : nat, express_relation n' (substitute_form [(n', make_numeral val)] f) (lift_relation n' pred val)
+  end
+.
+
+Example express_relation_example1 :
+  express_relation 2 (leq_form (ivar_tm 0) (ivar_tm 1)) (fun x0 : nat => fun x1 : nat => x0 <= x1).
+Proof.
+  simpl; intros val1 val2; constructor.
+  - intros x; apply orb_false_iff; constructor.
+    + eval_vr_eq_dec; simplify_make_numeral.
+    + eval_vr_eq_dec; simplify_make_numeral.
+  - constructor.
+    + intros H va.
+      eval_vr_eq_dec; simpl_eval_tm_make_numeral; tauto.
+    + intros H.
+      assert (H0 := H (fun _ : vr => 0)).
+      eval_in_vr_eq_dec H0; simpl_in_eval_tm_make_numeral H0; tauto.
+Qed.
+
+Fixpoint function_of_arity (n : nat) : Type :=
+  match n with
+  | 0 => nat
+  | S n' => nat -> function_of_arity n'
+  end
+.
+
+Fixpoint lift_function (n : nat) : function_of_arity (S n) -> nat -> function_of_arity n :=
+  match n as n0 return function_of_arity (S n0) -> nat -> function_of_arity n0 with
+  | 0 =>
+    fun func : nat -> nat =>
+    fun val : nat =>
+    func val
+  | S n' =>
+    fun func : nat -> nat -> function_of_arity n' =>
+    fun val : nat =>
+    fun val' : nat =>
+    lift_function n' (func val') val 
+  end
+.
+
+Fixpoint express_function (n : nat) : form -> function_of_arity n -> Prop :=
+  match n as n0 return form -> function_of_arity n0 -> Prop with
+  | 0 =>
+    fun f : form =>
+    fun func : nat =>
+    forall val : nat,
+    let f' : form := substitute_form [(0, make_numeral val)] f in
+    (forall x : vr, occursFreeIn_form x f' = false) /\ (val = func <-> forall va : value_assignment, eval_form va f')
+  | S n' =>
+    fun f : form =>
+    fun func : nat -> function_of_arity n' =>
+    forall val : nat, express_function n' (substitute_form [(n, make_numeral val)] f) (lift_function n' func val)
+  end
+.
+Ltac auto_show_it_is_sentence :=
+  tryif (apply orb_false_iff; constructor) then auto_show_it_is_sentence else (eval_vr_eq_dec; simplify_make_numeral)
+.
+
+Example express_function_example1 :
+  express_function 3 (eqn_form (ivar_tm 0) (plus_tm (ivar_tm 1) (plus_tm (ivar_tm 2) (ivar_tm 3)))) (fun x1 : nat => fun x2 : nat => fun x3 : nat => x1 + (x2 + x3)).
+Proof.
+  simpl; intros val3 val2 val1 val0; constructor.
+  - intros x; auto_show_it_is_sentence.
+  - constructor.
+    + intros H va.
+      eval_vr_eq_dec; simpl_eval_tm_make_numeral; tauto.
+    + intros H.
+      assert (H0 := H (fun _ : vr => 0)).
+      eval_in_vr_eq_dec H0; simpl_in_eval_tm_make_numeral H0; tauto.
+Qed.
+
 End Chapter2.
 
 End Smullyan's_Goedel's_Incompleteness_Theorems.
